Split out transition system and token machine from mfun

theories/TransitionSystem.v
@@ -1,280 +1,147 @@
-
-Section defn.
-  Context {State Arrow Result : Type}.
-
-  Class StrictTransitionSystem := {
-      ts_morph : Arrow -> relation State;
-      ts_terminal : State -> Result -> Prop;
-    }.
-
-  Class TransitionSystem `{StrictTransitionSystem} := {
-      ts_setoid :: Setoid State;
-      ts_morph_covariance : forall (a : Arrow), rel_covariant (ts_morph a);
-    }.
-
-  Definition compose `{StrictTransitionSystem} (a b : relation State) : relation State :=
-    fun s s'' =>
-      exists2 s', a s s' & b s' s''.
-End defn.
-
-Notation "A '~[' B ']~>' C" := (ts_morph B A C) (at level 20) : slot_scope.
-Infix "∘" := compose : slot_scope.
-
-Section leibniz_ts.
-  Context `{HSTS: StrictTransitionSystem}.
-
-  Program Instance leibnizTS : @TransitionSystem _ _ _ HSTS | 10 := {
-      ts_setoid := eq_setoid State;
-    }.
-  Next Obligation.
-    intros s s'1 s'2 Heq H. cbn in *. subst. now exists s'2.
-  Qed.
-End leibniz_ts.
-
-Open Scope slot_scope.
-
-Section props.
-  Context `{HTs: TransitionSystem}.
-
-  Theorem ts_compose_assoc (a b c : relation State) (s s' : State) :
-    (a ∘ (b ∘ c)) s s' <-> ((a ∘ b) ∘ c) s s'.
-    firstorder.
-  Qed.
-
-  Lemma compose_covariance (a b : relation State) (Hcov_a : rel_covariant a) (Hcov_b : rel_covariant b) :
-    rel_covariant (a ∘ b).
-  Proof.
-    intros s1 s2 s1'' Heq [s1' Hs1' Hs1''].
-    specialize (Hcov_a s1 s2 s1' Heq Hs1').
-    destruct Hcov_a as [s2' [Hs2' Heq']].
-    specialize (Hcov_b s1' s2' s1'' Heq' Hs1'').
-    destruct Hcov_b as [s2'' [Hs2'' Heq'']].
-    exists s2''. sauto.
-  Qed.
-
-  Definition commutative (a b : relation State) : Prop :=
-    forall s s',
-      (a ∘ b) s s' <-> (b ∘ a) s s'.
-
-  Definition setoid_commutative (a b : relation State) : Prop :=
-    forall s s1',
-      ((a ∘ b) s s1' -> exists{s2' == s1'}, (b ∘ a) s s2') /\
-      ((b ∘ a) s s1' -> exists{s2' == s1'}, (a ∘ b) s s2').
-End props.
-
-Fact eq_setoid_commutative `{HST : StrictTransitionSystem} :
-  forall a b,
-    commutative a b <-> @setoid_commutative _ _ _ HST leibnizTS a b.
-Proof.
-  split; unfold commutative, setoid_commutative.
-  - sauto.
-  - unfold compose, exists_equiv, equiv, ts_setoid, leibnizTS, eq_setoid.
-    intros H s s''. specialize (H s s'').
-    sauto.
-Qed.
+From Coq Require Import
+  Program
+  Decidable
+  List
+  Ensembles
+  Relation_Definitions
+  RelationClasses
+  SetoidClass
+  SetoidDec
+  Classes.Morphisms.
 
 Import ListNotations.
 
-Section trace.
-  Context `{HTS: TransitionSystem}.
+From Hammer Require Import
+  Tactics.
 
-  Inductive Trace : list Arrow -> State -> State -> Prop :=
-  | tr_nil : forall s,
-      Trace [] s s
-  | tr_cons : forall s s' s'' arrow trace,
-      s ~[arrow]~> s' ->
-      Trace trace s' s'' ->
-      Trace (arrow :: trace) s s''.
+From SLOT Require Import
+  Setoids
+  RestrictedPermutation
+  Multifunction
+  TokenMachine.
 
-  Fixpoint trace_via_compose (t : list (relation State)) : relation State :=
-    match t with
-    | [] => eq
-    | [a] => a
-    | (a :: t) => a ∘ trace_via_compose t
+Export Multifunction TokenMachine.
+
+Section TransitionSystem.
+  Context {State : Type}.
+
+  Definition ts_ret (Event : Type) := option (Event * State).
+
+  Definition ts_ret_setoid (Event : Type) (Hss : Setoid State) :=
+    let sp := @setoidPair Event State (eq_setoid _) Hss in
+    @setoid_option (Event * State) sp.
+
+  Class TransitionSystem {Event : Type} :=
+    {
+      ts_setoid :: Setoid State;
+      ts_canon_rel : relation Event;
+      ts_canon_order :: CanonicalOrder ts_canon_rel;
+      ts_state_trans :: @MFun State (ts_ret Event) ts_setoid (ts_ret_setoid Event ts_setoid);
+    }.
+
+  Program Definition ts_mfun `{TransitionSystem} (e : Event) : MFun State State :=
+    {| morphism s s' :=
+        s ~[ts_state_trans]~> Some (e, s');
+    |}.
+  Solve All Obligations with sauto.
+
+  Global Instance tsTokenSystem `{TransitionSystem} : @TokenMachine State Event :=
+    { tm_setoid := ts_setoid;
+      tm_canon_rel := ts_canon_rel;
+      tm_canon_order := ts_canon_order;
+      tm_state_trans := ts_mfun;
+    }.
+
+  Definition ts_event_commute `{TransitionSystem} (a b : Event) := commute (ts_mfun a) (ts_mfun b).
+End TransitionSystem.
+
+Section TSProps.
+  Context `{HTS : TransitionSystem}
+           (Hcanon_dec : forall f g : Event, decidable (ts_event_commute f g)).
+
+  (* TODO: this is an mfun *)
+  Inductive TSMFunGen : State -> list Event -> State -> Prop :=
+  | ts_nil : forall s,
+      s ~[ts_state_trans]~> None ->
+      TSMFunGen s [] s
+  | ts_cont : forall s s' s'' t event,
+      TSMFunGen s' t s'' ->
+      s ~[ts_state_trans]~> Some (event, s') ->
+      TSMFunGen s (event :: t) s''.
+
+  Lemma transition_system_as_token_machine_trace (s s' : State) (t : list Event) :
+    TSMFunGen s t s' ->
+      s ~[compose_list (map tm_state_trans t)]~> s'.
+  Proof.
+    intros.
+    induction H.
+    - reflexivity.
+    - destruct t; simpl in *.
+      + inversion H. now subst.
+      + exists s'. now split.
+  Qed.
+
+  Lemma tsfun_gen_as_te s s' : sufficient_replacement_p
+                                 (fun t => TSMFunGen s t s')
+                                 (fun t => exists{s'' == s'}, CanonicalTrace t s s'').
+  Proof.
+    intros t Ht.
+    apply transition_system_as_token_machine_trace in Ht.
+    now apply canonicalize_trace in Ht.
+  Qed.
+
+  Definition can_follow_ts (a b : Event) :=
+    event_commute a b -> ts_canon_rel a b.
+
+  Definition can_follow_hd_ts (token : Event) (trace : Trace) : Prop :=
+    match trace with
+    | [] => True
+    | head :: _ =>
+        can_follow_ts token head
     end.
 
-  Fact trace_is_compose_fold :
-    forall t s s',
-      Trace t s s' <-> trace_via_compose (map ts_morph t) s s'.
-  Proof with sauto.
-    intros t s s''.
-    split.
-    - intros Ht. induction Ht.
-      + easy.
-      + simpl in *.
-        destruct trace.
-        * sauto.
-        * simpl.
-          exists s'.
-          -- assumption.
-          -- apply IHHt.
-    - generalize dependent s. induction t; intros s Ht; simpl in Ht.
-      + rewrite Ht. constructor.
-      + destruct t; simpl in Ht.
-        * constructor 2 with (s' := s'')...
-        * inversion Ht.
-          specialize (IHt x).
-          constructor 2 with (s' := x); [assumption|].
-          simpl in IHt. apply IHt in H1.
-          assumption.
-  Qed.
-
-  Lemma trace_split : forall s s'' t1 t2,
-      Trace (t1 ++ t2) s s''  ->
-      exists s', Trace t1 s s' /\ Trace t2 s' s''.
-  Proof with sauto.
-    intros.
-    generalize dependent s.
-    induction t1; intros.
-    - exists s...
-    - simpl in H0. inversion H0. subst. clear H0.
-      destruct (IHt1 s' H6) as [s_ [Ht1 Ht2]].
-      exists s_. split; sauto.
-  Qed.
-
-  Lemma trace_concat : forall s s' s'' t1 t2,
-      Trace t1 s s' ->
-      Trace t2 s' s'' ->
-      Trace (t1 ++ t2) s s''.
-  Proof with sauto.
-    intros.
-    generalize dependent s.
-    induction t1...
-  Qed.
-
-  Lemma trace_equiv_covariance :
-    forall t, rel_covariant (Trace t).
+  Lemma can_follow_equiv a b : can_follow a b <-> can_follow_ts a b.
   Proof.
-    intros t.
-    induction t; intros s1 s2 s1' Hs12 Hs1'.
-    - inversion Hs1'. subst.
-      exists s2. split.
-      + constructor.
-      + assumption.
-    - inversion Hs1'; subst.
-      eapply ts_morph_covariance in H2; eauto.
-      destruct H2 as [s2_ [Hs2_ Heq]].
-      specialize (IHt s' s2_ s1' Heq H5).
-      destruct IHt as [s2' [Hs2' Heq']].
-      exists s2'; split.
-      + econstructor; eauto.
-      + assumption.
+    sauto.
   Qed.
 
-  Lemma trace_via_compose_eqiuv_covariance :
-    forall t, rel_covariant (trace_via_compose (map ts_morph t)).
+  Lemma can_follow_hd_equiv a t : can_follow_hd a t <-> can_follow_hd_ts a t.
   Proof.
-    intros t s s1 s2 s1' Ht.
-    rewrite <-trace_is_compose_fold in Ht.
-    eapply trace_equiv_covariance in Ht; eauto.
-    destruct Ht as [s2' [Hs2' Hs]]. exists s2'.
-    rewrite <-trace_is_compose_fold. easy.
+    sauto.
   Qed.
-End trace.
 
+  Inductive CanonicalTSMFunGen : State -> list Event -> State -> Prop :=
+  | cts_nil : forall s,
+      s ~[ts_state_trans]~> None ->
+      CanonicalTSMFunGen s [] s
+  | cts_cons : forall s s' s'' event trace,
+      s ~[ts_state_trans]~> Some (event, s') ->
+      can_follow_hd_ts event trace ->
+      CanonicalTSMFunGen s' trace s'' ->
+      CanonicalTSMFunGen s (event :: trace) s''.
 
-Definition morph_setoid_commutative `{TransitionSystem} a b := setoid_commutative (ts_morph a) (ts_morph b).
+  Lemma canon_ts_mfun_trace_is_always_canonical s s' t :
+    CanonicalTSMFunGen s t s' -> CanonicalTrace t s s'.
+  Proof.
+    intros H.
+    induction H.
+    - constructor.
+    - now constructor 2 with (s' := s').
+  Qed.
 
-Definition can_follow `{TransitionSystem} `{CanonicalOrder Arrow} (a b : Arrow) :=
-  (canon_rel a b = true) \/ (~morph_setoid_commutative a b).
-
-
-Definition TraceEnsemble {Arrow : Type} := Ensemble (list Arrow).
-
-Section trace_equivalence.
-  Context `{T : TransitionSystem} (e e' : @TraceEnsemble Arrow).
-
-  Definition sufficient_replacement :=
-    forall t s s'1, e t ->
-              Trace t s s'1 ->
-              exists t' s'2, e' t' /\ Trace t' s s'2 /\ s'1 == s'2.
-
-  Definition sufficient_replacement_p :=
-    forall t, e t ->
-         exists t', e' t' /\ RestrictedPermutation morph_setoid_commutative t t'.
-
-  Lemma trace_commut_swap2 a b s s'1 :
-    morph_setoid_commutative a b->
-    Trace [a; b] s s'1 ->
-    exists{s'2 == s'1}, Trace [b; a] s s'2.
+  Theorem canonicalize_transition_system : forall s s' t,
+      TSMFunGen s t s' ->
+      exists t', exists{s'' == s'},
+        CanonicalTSMFunGen s t' s''.
   Proof.
     intros.
-    apply trace_is_compose_fold in H1. simpl in H1.
-    destruct (H0 s s'1) as [Hcomm _].
-    destruct (Hcomm H1) as [s'2 [H2 Hs'2]].
-    exists s'2. split.
-    - now rewrite trace_is_compose_fold.
-    - assumption.
-  Qed.
-
-  Lemma trace_commutative_permutation s s'1 t t' :
-    Trace t s s'1 ->
-    RestrictedPermutation morph_setoid_commutative t t' ->
-    exists{s'2 == s'1}, Trace t' s s'2.
-  Proof with easy.
-    intros Hls Hperm.
-    generalize dependent s. generalize dependent s'1.
-    induction Hperm; intros.
-    - exists s. sauto.
-    - inversion Hls; subst; clear Hls.
-      specialize (IHHperm s'1 s' H5).
-      destruct IHHperm as [s'2 [Hs'2 Hl2]].
-      exists s'2; split.
-      + now constructor 2 with (s' := s').
-      + assumption.
-    - replace (a :: b :: l) with ([a; b] ++ l) in Hls by reflexivity.
-      replace (b :: a :: l) with ([b; a] ++ l) by reflexivity.
-      apply trace_split in Hls. destruct Hls as [s' [Hab Hls]].
-      apply trace_commut_swap2 in Hab; [|assumption].
-      destruct Hab as [s_ [Hsl_ Hs_]].
-      specialize (trace_equiv_covariance l s' s_ s'1 Hs_ Hls) as Hls_.
-      destruct Hls_ as [s'2 [Hls_ Hs'2]].
-      exists s'2. split; [|assumption].
-      apply trace_concat with (s' := s_)...
-    - specialize (IHHperm1 s'1 s Hls).
-      destruct IHHperm1 as [s'2 [Hls'2 Hs'2]].
-      specialize (IHHperm2 s'2 s Hls'2).
-      destruct IHHperm2 as [s'3 [Hls'3 Hs'3]].
-      exists s'3. split.
-      + assumption.
-      + rewrite Hs'2...
-  Qed.
-
-  (* Lemma comm_perm_sufficient_replacement : *)
-  (*   sufficient_replacement_p -> *)
-  (*   sufficient_replacement. *)
-  (* Proof. *)
-  (*   intros Hsrp t s s'1 Het Hs'1. *)
-  (*   specialize (Hsrp t Het). clear Het. *)
-  (*   destruct Hsrp as [t' [He't' Hperm]]. *)
-  (*   generalize dependent s. generalize dependent s'1. *)
-  (*   induction Hperm; intros s s'1 Ht. *)
-  (*   - sauto. *)
-  (*   -  *)
-
-
-
-
-    -
-    induction Hperm.
-    - intros s s'1 He_t Hs'1.
-      exists []. exists s.
-      inversion Hs'1; subst.
-      repeat split.
-      +
-
-    intros Hsrp t s s' Ht Hls.
-    destruct (Hsrp t Ht) as [t' [Ht' Hperm]].
-    induction Hperm.
-    - exists []. exists s. repeat split.
-      + assumption.
-      + constructor.
-      + inversion Hls. apply reflexivity.
-    - inversion Hls; subst; clear Hls.
-      assert (e l1). {
-
-      specialize (IHHperm
-
-    eapply trace_commutateive_permutation in Hperm; eauto.
-  Qed.
-End trace_equivalence.
+    specialize (transition_system_as_token_machine_trace s s' t H) as Hss'.
+    specialize (canonicalize_trace Hcanon_dec s s' t) as Hcan.
+    simpl in Hcan. apply Hcan in Hss'. clear Hcan.
+    destruct Hss' as [t' Ht'].
+    exists t'.
+    destruct Ht' as [[s'' [Hss'' Heq]] Ht'].
+    exists s''.
+    split; [|assumption].
+  Abort.
+End TSProps.
